chore: remove indices from mutual inductives

Reflection/MutualInductive.lean
@@ -13,7 +13,7 @@ set_option pp.proofs true
 /-- Example for `Nat` is `U`, for `Vec` is `SPi Nat (fun n => U)`. -/
 inductive Tyₛ : Type (u+1)
 | U : Tyₛ
-| SPi : (T : Type u) -> (T -> Tyₛ) -> Tyₛ
+-- | SArr : (T : Type u) -> Tyₛ -> Tyₛ
 open Tyₛ
 
 inductive Conₛ
@@ -47,7 +47,7 @@ inductive Tmₛ.{u} : Conₛ.{u} -> Tyₛ.{u} -> Type (u+1)
 -------------------------------------app-Intro
 Γ ⊢ₛ f arg : A arg
 ``` -/
-| app : Tmₛ Γ (SPi T A) -> (arg : T) -> Tmₛ Γ (A arg)
+-- | app : Tmₛ Γ (SArr T A) -> (arg : T) -> Tmₛ Γ A
 infixl:50 " @ " => Tmₛ.app
 
 -- -- ! This fails:
@@ -70,11 +70,11 @@ For example the variables are `Even` and `Odd`, i.e. the other types in the mutu
 then `Even @ 123` is a term in universe `U`. -/
 inductive Tyₚ : Conₛ -> Type (u+1)
 | El : Tmₛ Γₛ U -> Tyₚ Γₛ
-| PPi   : (T : Type u) -> (T -> Tyₚ Γₛ) -> Tyₚ Γₛ
+| PArr   : (T : Type u) -> Tyₚ Γₛ -> Tyₚ Γₛ
 /-- Allows us to introduce nested binders `(x : Self ...) -> ...`.
   `PFunc` is non-dependent, because it makes no sense to have `(self : Self ...) -> Self self`.
   (...but once you have ind-ind or ind-rec, it might be sensible?) -/
-| PFunc : Tmₛ Γₛ U   ->       Tyₚ Γₛ  -> Tyₚ Γₛ
+| PFunc : Tmₛ Γₛ U   -> Tyₚ Γₛ  -> Tyₚ Γₛ
 open Tyₚ
 
 /-- List of constructor descriptions.
@@ -99,18 +99,17 @@ section Examples
   /-- Corresponds to the two constructors `Nat.zero : Nat` and `Nat.succ : Nat -> Nat`. -/
   def N  : Conₚ Nₛ := El (.var .vz) :: PFunc (.var .vz) (El (.var .vz)) :: []
 
-  -- Vec : Nat -> U
-  def Vₛ : Conₛ := SPi Nat (fun _ => U) :: []
+  -- List : U
+  def Vₛ : Conₛ := U :: []
 
-  -- Vec : Nat -> U   ⊢ₛ   Vec 0 : U
-  def V_nil : Tyₚ Vₛ := El ((.var .vz) @ 0) -- Vec 0
+  -- Vec : Nat -> U   ⊢ₛ  List A : U
+  def V_nil : Tyₚ Vₛ := El (.var .vz) -- Vec 0
 
-  -- Vec : Nat -> U   ⊢ₛ   (n : Nat) -> A -> Vec n -> Vec (n + 1)
+  -- cons : Nat -> U   ⊢ₛ  A → List A → List A
   def V_cons {A : Type} : Tyₚ Vₛ :=
-    PPi Nat fun n => -- (n : Nat) ->
-      PPi A fun _ => -- A ->
-        PFunc ((Tmₛ.var vz) @ n) <| -- Vec n ->
-          El ((Tmₛ.var vz) @ (n + 1)) -- Vec (n + 1)
+    PArr A <| -- A →
+      PFunc (Tmₛ.var vz) <| -- List A ->
+        El (Tmₛ.var vz) -- List A
 
   def V (A : Type) : Conₚ Vₛ := V_nil :: @V_cons A :: []
 end Examples
@@ -120,14 +119,14 @@ end Examples
 /-- Interprets a sort type, for example `SPi Nat (fun n => U)` becomes `Nat -> Type`. -/
 def TyₛA.{u, v} : Tyₛ.{u} -> Type ((max u v) + 1)
 | U => Type (max u v)
-| SPi T A => (t : T) -> TyₛA (A t)
+-- | SPi T A => (t : T) -> TyₛA (A t)
 
 /-- Interprets a context of type formers.  The `Vec` example becomes `(Nat -> Type) × Unit`. -/
 def ConₛA.{u, v} : Conₛ.{u} -> Type ((max u v) + 1)
 | .nil => PUnit.{(max u v) + 2}
 | .cons A Γ => Prod.{(max u v) + 1} (TyₛA.{u, v} A) (ConₛA Γ)
 
-example : ConₛA Vₛ = ((Nat -> Type) × PUnit.{2}) := by rfl
+example : ConₛA Vₛ = (Type × PUnit.{2}) := by rfl
 
 /--
   Variable lookup. Given a context `Γₛ` and an interpretation `γₛ` for that context,
@@ -170,13 +169,13 @@ _ᵃt : ∀{ℓ Γc B} → TmS Γc B → _ᵃc {ℓ} Γc → _ᵃS {ℓ} B
 ```
 -/
 def TmₛA.{u} : {Γₛ : Conₛ.{u}} -> {Aₛ : Tyₛ} -> Tmₛ Γₛ Aₛ -> ConₛA Γₛ -> TyₛA.{u} Aₛ
-| Γ, A, @Tmₛ.var _   _ v  , γₛ => VarₛA v γₛ
-| Γ, _, @Tmₛ.app Γ T A t u, γₛ => (TmₛA t γₛ) u
+| _Γ, _A, @Tmₛ.var _   _ v  , γₛ => VarₛA v γₛ
+-- | Γ, _, @Tmₛ.app Γ T A t u, γₛ => (TmₛA t γₛ) u
 
 @[simp] theorem TmₛA_var  : TmₛA (Tmₛ.var v) γₛ = VarₛA v γₛ := by rw [TmₛA]
-@[simp] theorem TmₛA_app  : TmₛA (Tmₛ.app t u) γₛ = (TmₛA t γₛ) u := by rw [TmₛA]
+-- @[simp] theorem TmₛA_app  : TmₛA (Tmₛ.app t u) γₛ = (TmₛA t γₛ) u := by rw [TmₛA]
 
-example {Vec : Nat -> Type} : @TmₛA (SPi Nat (fun _ => U) :: []) U ((.var .vz) @ 123) ⟨Vec, ⟨⟩⟩ = Vec 123 := rfl
+example {Vec : Type} : @TmₛA (U :: []) U (.var .vz) ⟨Vec, ⟨⟩⟩ = Vec := rfl
 
 /-- Interprets a constructor type. See below for examples.  Example:
 ```
@@ -188,17 +187,17 @@ reduces to the type of `Vec.cons` as you would expect:
 ``` -/
 def TyₚA.{u, v} : Tyₚ.{u} Γₛ -> ConₛA.{u, v} Γₛ -> Type (max u v)
 | El         Self, γₛ => TmₛA Self γₛ
-| PPi   T    Rest, γₛ => (arg : T)    -> TyₚA (Rest arg) γₛ
+| PArr   T    Rest, γₛ => (arg : T)    -> TyₚA Rest γₛ
 | PFunc Self Rest, γₛ => TmₛA Self γₛ -> TyₚA Rest γₛ
 
-example {Vec : Nat -> Type} {_A : Type}
+example {Vec : Type} {_A : Type}
   : TyₚA V_nil ⟨Vec, ⟨⟩⟩
-  = Vec 0
+  = Vec
   := rfl
 
-example {Vec : Nat -> Type} {A : Type}
+example {Vec : Type} {A : Type}
   : TyₚA (@V_cons A) ⟨Vec, ⟨⟩⟩
-  = ((n : Nat) -> A -> Vec n -> Vec (n + 1))
+  = (A -> Vec -> Vec)
   := rfl
 
 /-- Interprets a (mutual) inductive type. This is just `TyₚA` for each ctor joined with `×`.
@@ -216,9 +215,9 @@ def ConₚA.{u, v} : Conₚ.{u} Γₛ -> ConₛA.{u, v} Γₛ -> Type (max u v)
 | .nil, _ => PUnit
 | .cons A Γ, γₛ => TyₚA.{u, v} A γₛ × ConₚA Γ γₛ
 
-example {Vec : Nat -> Type} {A : Type}
+example {Vec : Type} {A : Type}
   : ConₚA (V A) ⟨Vec, ⟨⟩⟩
-  = ((Vec 0) × ((n : Nat) -> A -> Vec n -> Vec (n + 1)) × Unit)
+  = (Vec × (A -> Vec -> Vec) × Unit)
   := rfl
 
 -- ## Displayed Algebras
@@ -228,7 +227,7 @@ example {Vec : Nat -> Type} {A : Type}
 Example: `TyₛD (SPi Nat (fun _ => U)) Vec` reduces to `(n : Nat) -> Vec n -> Type`. -/
 def TyₛD.{u, v} : (Aₛ : Tyₛ.{u}) -> TyₛA.{u, v} Aₛ -> Type ((max u v) + 1)
 | U, T => T -> Type (max u v)
-| SPi T Aₛ, f => (t : T) -> TyₛD (Aₛ t) (f t)
+-- | SPi T Aₛ, f => (t : T) -> TyₛD (Aₛ t) (f t)
 
 /-- Compute motive type for each mutually defined inductive type.
 
@@ -244,7 +243,7 @@ def ConₛD.{u, v} : (Γₛ : Conₛ.{u}) -> ConₛA.{u, v} Γₛ -> Type ((max 
 | .nil, _ => PUnit
 | .cons A Γ, ⟨a, γ⟩ => TyₛD A a × ConₛD Γ γ
 
-example {Vec : Nat -> Type} : ConₛD Vₛ ⟨Vec, ⟨⟩⟩ = (((t : Nat) → Vec t -> Type) × PUnit.{2}) := rfl
+example {Vec : Type} : ConₛD Vₛ ⟨Vec, ⟨⟩⟩ = ((Vec -> Type) × PUnit.{2}) := rfl
 
 def VarₛD : (v : Varₛ Γₛ Aₛ) -> ConₛD Γₛ γₛ -> TyₛD Aₛ (VarₛA v γₛ)
 | .vz  , ⟨a, _⟩ => a
@@ -262,11 +261,11 @@ for this is, again with `VarₛD` inlined:
 -- ! TmₛD needs casts because reduction behaviour of TmₛA is broken.
 -- And for some reason TmₚD works just fine? What...
 def TmₛD : {Γₛ : Conₛ} -> {Aₛ : Tyₛ} -> {γₛ : ConₛA Γₛ} -> (t : Tmₛ  Γₛ Aₛ) -> ConₛD Γₛ γₛ -> TyₛD Aₛ (TmₛA t γₛ)
-|  _, _, γₛ, .var v                    , γₛD => TmₛA_var.symm ▸ VarₛD v γₛD
-| Γₛ, _, γₛ, .app (T := T) (A := A) t u, γₛD => TmₛA_app.symm ▸ TmₛD t γₛD u
+|  _, _, _γₛ, .var v                    , γₛD => TmₛA_var.symm ▸ VarₛD v γₛD
+-- | Γₛ, _, γₛ, .app (T := T) (A := A) t u, γₛD => TmₛA_app.symm ▸ TmₛD t γₛD u
 
 theorem TmₛD_var : TmₛD (Tmₛ.var v) γₛD = TmₛA_var.symm ▸ VarₛD v γₛD := by rw [TmₛD]
-theorem TmₛD_app : TmₛD (t @ u)     γₛD = TmₛA_app.symm ▸ TmₛD t γₛD u := by rw [TmₛD]
+-- theorem TmₛD_app : TmₛD (t @ u)     γₛD = TmₛA_app.symm ▸ TmₛD t γₛD u := by rw [TmₛD]
 
 /-- Example:
 ```
@@ -280,21 +279,21 @@ Example:
 ``` -/
 -- Note: The `Self` here can be a little misleading, as it may be a nested type with different indices.
 def TyₚD.{u, v} : (A : Tyₚ.{u} Γₛ) -> ConₛD.{u} Γₛ γₛ -> TyₚA.{u, v} A γₛ -> Type (max u v)
-| El         Self, γD, self =>                                               TmₛD Self γD self
-| PPi   T    Rest, γD, f    => (t : T) ->                                    TyₚD (Rest t) γD (f t)
+| El         Self, γD, self => TmₛD Self γD self
+| PArr   T    Rest, γD, f   => (t : T) -> TyₚD Rest γD (f t)
 | PFunc Self Rest, γD, f    => ⦃self : TmₛA Self γₛ⦄ -> TmₛD Self γD self -> TyₚD Rest γD (f self)
 
 inductive Vec (A : Type) : Nat -> Type
 | nil : Vec A 0
 | cons : (n : Nat) -> A -> Vec A n -> Vec A (n + 1)
 
-example {A : Type} {P : (n : Nat) -> Vec A n -> Type}
-  : @TyₚD Vₛ ⟨Vec A, ⟨⟩⟩ V_nil ⟨P, ⟨⟩⟩ Vec.nil
-  = P 0 Vec.nil
+example {A : Type} {P : List A -> Type}
+  : @TyₚD Vₛ ⟨List A, ⟨⟩⟩ V_nil ⟨P, ⟨⟩⟩ List.nil
+  = P List.nil
   := rfl
-example {A : Type} {P : (n : Nat) -> Vec A n -> Type}
-  : @TyₚD Vₛ ⟨Vec A, ⟨⟩⟩ V_cons ⟨P, ⟨⟩⟩ Vec.cons
-  = ((n : Nat) -> (a : A) -> (v : Vec A n) -> P n v -> P (n + 1) (Vec.cons n a v))
+example {A : Type} {P : List A -> Type}
+  : @TyₚD Vₛ ⟨List A, ⟨⟩⟩ V_cons ⟨P, ⟨⟩⟩ List.cons
+  = ((a : A) -> (v : List A) -> P v -> P (List.cons a v))
   := rfl
 
 /-- Example:
@@ -311,11 +310,11 @@ def ConₚD.{u, v} : (Γ : Conₚ.{u} Γₛ) -> ConₛD.{u, v} Γₛ γₛ -> Co
 | .nil, _, _ => PUnit
 | .cons A Γ, γD, ⟨a, γ⟩ => TyₚD A γD a × ConₚD Γ γD γ
 
-example {P : (n : Nat) -> Vec A n -> Type}
-  : @ConₚD Vₛ ⟨Vec A, ⟨⟩⟩ (V_nil :: V_cons :: []) ⟨P, ⟨⟩⟩ ⟨Vec.nil, Vec.cons, ⟨⟩⟩
+example {P : List A -> Type}
+  : @ConₚD Vₛ ⟨List A, ⟨⟩⟩ (V_nil :: V_cons :: []) ⟨P, ⟨⟩⟩ ⟨List.nil, List.cons, ⟨⟩⟩
   = (
-        (P 0 Vec.nil)
-      × ((n : Nat) -> (a : A) -> (v : Vec A n) -> P n v -> P (n + 1) (Vec.cons n a v))
+        (P List.nil)
+      × ((a : A) -> (v : List A) -> P v -> P (List.cons a v))
       × Unit
     )
   := rfl
@@ -334,9 +333,9 @@ reduces to
 ``` -/
 def TyₛS.{u, v} : (Aₛ : Tyₛ.{u}) -> (αₛ : TyₛA.{u, v} Aₛ) -> TyₛD.{u, v} Aₛ αₛ -> Type (max u v)
 | U       , T , TD  => (t : T) -> TD t
-| SPi T Aₛ, fₛ, fₛd => (t : T) -> TyₛS (Aₛ t) (fₛ t) (fₛd t)
+-- | SPi T Aₛ, fₛ, fₛd => (t : T) -> TyₛS (Aₛ t) (fₛ t) (fₛd t)
 
-example {A R} : TyₛS (SPi Nat (fun _ => U)) (Vec A) (fun _ _ => R) = ((n : Nat) -> (v : Vec A n) -> R) := rfl
+-- example {A R} : TyₛS (SPi Nat (fun _ => U)) (Vec A) (fun _ _ => R) = ((n : Nat) -> (v : Vec A n) -> R) := rfl
 
 /-- Example:
 ```
@@ -351,7 +350,7 @@ def ConₛS.{u, v} : (Γₛ : Conₛ.{u}) -> (γₛ : ConₛA.{u, v} Γₛ) -> C
 | .nil, ⟨⟩, ⟨⟩ => PUnit
 | .cons Aₛ Γₛ, ⟨αₛ, γₛ⟩, ⟨αₛd, γₛd⟩ => TyₛS Aₛ αₛ αₛd × ConₛS Γₛ γₛ γₛd
 
-example {A R} : ConₛS Vₛ ⟨Vec A, ⟨⟩⟩ ⟨fun _ _ => R, ⟨⟩⟩ = (((n : Nat) -> (v : Vec A n) -> R) × Unit) := rfl
+-- example {A R} : ConₛS Vₛ ⟨Vec A, ⟨⟩⟩ ⟨fun _ _ => R, ⟨⟩⟩ = (((n : Nat) -> (v : Vec A n) -> R) × Unit) := rfl
 
 def VarₛS : (x : Varₛ Γₛ Aₛ) -> ConₛS Γₛ γₛ γD -> TyₛS Aₛ (VarₛA x γₛ) (VarₛD x γD)
 | .vz  , ⟨αₛS, γₛS⟩ => αₛS
@@ -368,14 +367,10 @@ def TmₛS : {Γₛ : Conₛ} -> {Aₛ : Tyₛ} -> {γₛ : ConₛA Γₛ} -> {�
   have hA : TmₛA (Tmₛ.var v) γₛ = VarₛA v γₛ := TmₛA_var
   rw [TyₛS_helper hA (TmₛD (Tmₛ.var v) γₛD), TmₛD_var, eq_symm_cancel hA]
   exact VarₛS v γₛS
-| Γₛ, _, γₛ, γₛD, .app (T := T) (A := Aₛ) t u, γₛS => by
-  have hA : TmₛA (Tmₛ.app t u) γₛ = TmₛA t γₛ u := TmₛA_app
-  rw [TyₛS_helper hA, TmₛD, eq_symm_cancel hA]
-  exact TmₛS t γₛS u
 
 def TyₚS : (A : Tyₚ Γₛ) -> ConₛS Γₛ γₛ γₛD -> (α : TyₚA A γₛ) -> TyₚD A γₛD α -> Prop
 | El         Self, γₛS, α, αD =>                          TmₛS Self γₛS α = αD -- note the equality here!
-| PPi   T    Rest, γₛS, f, fD => (t    : T)            -> TyₚS (Rest t) γₛS (f t)    (fD t)
+| PArr   T    Rest, γₛS, f, fD => (t    : T)         -> TyₚS Rest γₛS (f t)    (fD t)
 | PFunc Self Rest, γₛS, f, fD => (self : TmₛA Self γₛ) ->
   -- fD : {self : TmₛA Self γₛ} → TmₛD Self γD self → TyₚD Rest γD (f self)
   TyₚS  Rest    γₛS (f self) (@fD self (TmₛS Self γₛS self))
@@ -384,11 +379,11 @@ def ConₚS : (Γ : Conₚ Γₛ) -> ConₛS Γₛ γₛ γₛD -> (γ : ConₚA
 | .nil     ,   _,     ⟨⟩,       ⟨⟩ => True
 | .cons A Γ, γₛS, ⟨α, γ⟩, ⟨αD, γD⟩ => TyₚS A γₛS α αD ∧ ConₚS Γ γₛS γ γD
 
-example : @ConₚS Vₛ ⟨Vec A, ⟨⟩⟩ ⟨Q, ⟨⟩⟩ (V A) ⟨f, ⟨⟩⟩ ⟨Vec.nil, Vec.cons, ⟨⟩⟩ ⟨nilD, consD, ⟨⟩⟩
-  = (f 0 Vec.nil = nilD
-    ∧ ((n : Nat) -> (a : A) -> (v : Vec A n) -> (f (n + 1) (Vec.cons n a v) = consD n a /- v -/ (f n v)))
-    ∧ True)
-  := rfl
+-- example : @ConₚS Vₛ ⟨Vec A, ⟨⟩⟩ ⟨Q, ⟨⟩⟩ (V A) ⟨f, ⟨⟩⟩ ⟨Vec.nil, Vec.cons, ⟨⟩⟩ ⟨nilD, consD, ⟨⟩⟩
+--   = (f 0 Vec.nil = nilD
+--     ∧ ((n : Nat) -> (a : A) -> (v : Vec A n) -> (f (n + 1) (Vec.cons n a v) = consD n a /- v -/ (f n v)))
+--     ∧ True)
+--   := rfl
 
 
 -- # Substitutions
@@ -409,11 +404,11 @@ def SubₛVar : Varₛ Δₛ Aₛ -> Subₛ Γₛ Δₛ -> Tmₛ Γₛ Aₛ
 /-- Applies the substitution to a term, resulting in a new term in the new context. -/
 def SubₛTm : {Aₛ : _} -> Tmₛ Δₛ Aₛ -> Subₛ Γₛ Δₛ -> Tmₛ Γₛ Aₛ
 | _, .var v, σ => SubₛVar v σ
-| _, .app (A := _A) t u, σ => .app (SubₛTm t σ) u
+-- | _, .app (A := _A) t u, σ => .app (SubₛTm t σ) u
 
 def SubₛTy : Tyₚ Δₛ -> Subₛ Γₛ Δₛ -> Tyₚ Γₛ
 | El Self, σ => El (SubₛTm Self σ)
-| PPi T Rest, σ => PPi T (fun t => SubₛTy (Rest t) σ)
+| PArr T Rest, σ => PArr T (SubₛTy Rest σ)
 | PFunc Self Rest, σ => PFunc (SubₛTm Self σ) (SubₛTy Rest σ)
 
 def SubₛCon : Conₚ Δₛ -> Subₛ Γₛ Δₛ -> Conₚ Γₛ
@@ -423,7 +418,7 @@ def SubₛCon : Conₚ Δₛ -> Subₛ Γₛ Δₛ -> Conₚ Γₛ
 /-- Increment all de brujin indices in this term by one. -/
 def vshift : {Aₛ : Tyₛ} -> Tmₛ Γₛ Aₛ -> Tmₛ (Bₛ :: Γₛ) Aₛ
 | _, .var v => .var (.vs v)
-| _, .app (A := _A) t u => .app (vshift t) u
+-- | _, .app (A := _A) t u => .app (vshift t) u
 
 /-- Weakens a substitution.
   Given a substitution `σ` which replaces all variables `Δₛ ⊢ v` with terms `Γₛ ⊢ t`,
@@ -448,7 +443,7 @@ theorem aux : @Eq (Tmₛ (Bₛ :: Γₛ) Aₛ) (vshift (SubₛVar v (Subₛ.id �
       := congrArg vshift ih.symm
     simp only [SubₛVar]
     simp only [Subₛ.id, weaken, vshift, SubₛVar]
-    rw [h]
+    -- rw [h]
     -- simp [<- ih]
     -- rw [ih] at h
     sorry
@@ -469,7 +464,7 @@ theorem SubₛVar_id : (v : Varₛ Γₛ Aₛ) -> SubₛVar v (Subₛ.id Γₛ) 
 
 theorem SubₛTm_id : (t : Tmₛ Γₛ Aₛ) -> SubₛTm t (Subₛ.id Γₛ) = t
 | .var v => SubₛVar_id v
-| .app (A := Aₛ) t u => sorry
+-- | .app (A := Aₛ) t u => sorry
 
 def SubₛA : Subₛ Γₛ Δₛ -> ConₛA Γₛ -> ConₛA Δₛ
 | .nil     ,  _ => ⟨⟩
@@ -493,7 +488,7 @@ inductive Varₚ : Conₚ Γₛ -> Tyₚ Γₛ -> Type (u+1)
 set_option genInjectivity false in
 inductive Tmₚ.{u} {Γₛ : Conₛ.{u}} : Conₚ.{u} Γₛ -> Tyₚ.{u} Γₛ -> Type (u+1)
 | var : Varₚ Γ A -> Tmₚ Γ A
-| app {T : Type u} {A : T -> Tyₚ Γₛ} : Tmₚ Γ (PPi T A)   -> (t : T)      -> Tmₚ Γ (A t)
+| app {T : Type u} {A : Tyₚ Γₛ} : Tmₚ Γ (PArr T A)   -> (t : T)      -> Tmₚ Γ A
 | appr             {A :      Tyₚ Γₛ} : Tmₚ Γ (PFunc a A) -> Tmₚ Γ (El a) -> Tmₚ Γ A
 
 /-- Represents a substitution from Δₛ to Γₛ.
@@ -587,16 +582,16 @@ We do not have an actual `Vec String`, so instead we use `constrTmₛ (V String)
 -/
 def constrTmₛ' : {Aₛ : Tyₛ.{u}} -> Tmₛ.{u} Ωₛ Aₛ -> TyₛA.{u, u + 1} Aₛ -- baked-in ULift into TyₛA
 | U      , t => Tmₚ Ω (El t)
-| SPi _ _, t => fun u => constrTmₛ' (.app t u)
+-- | SArr _ _, t => fun u => constrTmₛ' (.app t u)
 
 #reduce TyₛA U
-example : TyₛA.{0, 1} U := constrTmₛ' (Ω := V String) (Ωₛ := Vₛ) ((.var .vz) @ 123)
-#reduce TyₛA (SPi Nat (fun _ => U))
-example : TyₛA (SPi Nat (fun _ => U)) := constrTmₛ' (Ω := V String) (Ωₛ := Vₛ) (.var .vz)
+-- example : TyₛA.{0, 1} U := constrTmₛ' (Ω := V String) (Ωₛ := Vₛ) ((.var .vz) @ 123)
+-- #reduce TyₛA (SPi Nat (fun _ => U))
+-- example : TyₛA (SPi Nat (fun _ => U)) := constrTmₛ' (Ω := V String) (Ωₛ := Vₛ) (.var .vz)
 
-example : constrTmₛ' (Ω := V String) (Ωₛ := Vₛ) (Aₛ := (SPi Nat (fun _ => U))) (.var .vz)
-  = fun (n : Nat) => Tmₚ (V String) (El ((.var .vz) @ n))
-  := rfl
+-- example : constrTmₛ' (Ω := V String) (Ωₛ := Vₛ) (Aₛ := (SPi Nat (fun _ => U))) (.var .vz)
+--   = fun (n : Nat) => Tmₚ (V String) (El ((.var .vz) @ n))
+--   := rfl
 
 def constrₛ' : Subₛ Ωₛ Γₛ -> ConₛA Γₛ
 | .nil => ⟨⟩
@@ -604,9 +599,9 @@ def constrₛ' : Subₛ Ωₛ Γₛ -> ConₛA Γₛ
 
 def constrₛ : ConₛA Ωₛ := constrₛ' (Ω := Ω) (Subₛ.id Ωₛ)
 
-example : constrₛ (Ωₛ := Vₛ) (Ω := V String)
-  = ⟨fun u => Tmₚ (V String) (El ((Tmₛ.var .vz) @ u)), ⟨⟩⟩
-  := rfl
+-- example : constrₛ (Ωₛ := Vₛ) (Ω := V String)
+--   = ⟨fun u => Tmₚ (V String) (El ((Tmₛ.var .vz) @ u)), ⟨⟩⟩
+--   := rfl
 
 -- Lemma 16
 theorem constrₛ_coherent (t : Tmₛ Γₛ Aₛ) (σ : Subₛ Ωₛ Γₛ) : TmₛA t (@constrₛ' Ωₛ Ω Γₛ σ) = @constrTmₛ' Ωₛ Ω _ (SubₛTm t σ) := by
@@ -619,37 +614,31 @@ theorem constrₛ_coherent (t : Tmₛ Γₛ Aₛ) (σ : Subₛ Ωₛ Γₛ) : Tm
       | vz =>
         rw [TmₛA]
         rw [constrₛ']
-        rw [VarₛA]
+        -- rw [VarₛA]
         rfl
       | vs v =>
         rw [TmₛA]
         rw [constrₛ']
-        rw [VarₛA]
+        -- rw [VarₛA]
         -- rw [constrTmₛ']
         -- rw [ih_σ]
         sorry
         done
-    | app f u ihₜ =>
-      rw [TmₛA]
-      rw [SubₛTm]
-      -- rw [ihₜ (f)]
-      -- rw [constrTmₛ']
-      sorry
-      done
+
 
 -- same as the above
 example (t : Tmₛ Γₛ Aₛ) : (TmₛA t) ∘ (@constrₛ' Ωₛ Ω Γₛ) = (@constrTmₛ' Ωₛ Ω _) ∘ (SubₛTm t)
   := funext <| constrₛ_coherent t
 
-example
-  : @TyₚA Vₛ (PPi Nat fun n => @El Vₛ ((.var vz) @ n)) (@constrₛ Vₛ (V String))
-  -- = ((n : Nat) -> (fun n => Tmₚ (V String) (El ((.var .vz) @ n))) n) -- intermediate step
-  = ((n : Nat) -> Tmₚ (V String) (El ((.var .vz) @ n)))
-  := rfl
-example --       vvvvvvvvvvvvvvvvvv "Self"
-  : @TyₚA Vₛ (El ((.var vz) @ 123)) (@constrₛ Vₛ (V String))
-  = Tmₚ (V String) (El ((.var .vz) @ 123))
-  := rfl
+-- example
+--   : @TyₚA Vₛ (PPi Nat fun n => @El Vₛ ((.var vz) @ n)) (@constrₛ Vₛ (V String))
+--   -- = ((n : Nat) -> (fun n => Tmₚ (V String) (El ((.var .vz) @ n))) n) -- intermediate step
+--   = ((n : Nat) -> Tmₚ (V String) (El ((.var .vz) @ n)))
+--   := rfl
+-- example --       vvvvvvvvvvvvvvvvvv "Self"
+--   : @TyₚA Vₛ (El ((.var vz) @ 123)) (@constrₛ Vₛ (V String))
+--   = Tmₚ (V String) (El ((.var .vz) @ 123))
+--   := rfl
 
 def constrTmₚ' : {A : Tyₚ _} -> Tmₚ Ω A -> TyₚA A (constrₛ (Ω := Ω))
 | El Self, t => by
@@ -659,7 +648,7 @@ def constrTmₚ' : {A : Tyₚ _} -> Tmₚ Ω A -> TyₚA A (constrₛ (Ω := Ω)
   rw [constrₛ_coherent Self]
   rw [SubₛTm_id]
   exact t
-| PPi T A, t => fun τ => constrTmₚ' (.app t τ)
+| PArr T A, t => fun τ => constrTmₚ' (.app t τ)
 | PFunc Self A, t =>
   fun u =>
     let u : Tmₚ Ω (El Self) := by
@@ -693,14 +682,14 @@ def elimTmₛ' : {Aₛ : Tyₛ.{u}} -> (t : Tmₛ.{u} Ωₛ Aₛ) -> TyₛS.{u, 
     -- ⊢ TmₛD a ωₛD t
     -- let ret := TmₛD t ωₛD
     sorry
-| SPi T Aₛ, t =>
-  fun τ => by
-    let res := elimTmₛ' (.app t τ)
-    -- why is this so ass
-    rw [TyₛS_helper TmₛA_app] at res
-    rw [TmₛD_app] at res
-    simp only [eq_symm_cancel, eq_cast_trans] at res
-    exact res
+-- | SPi T Aₛ, t =>
+--   fun τ => by
+--     let res := elimTmₛ' (.app t τ)
+--     -- why is this so ass
+--     rw [TyₛS_helper TmₛA_app] at res
+--     rw [TmₛD_app] at res
+--     simp only [eq_symm_cancel, eq_cast_trans] at res
+--     exact res
 
 def elimₛ' : (σ : Subₛ Ωₛ Γₛ) -> ConₛS Γₛ (SubₛA σ constrₛ) (SubₛD σ ωₛD)
 | .nil => ⟨⟩
@@ -712,10 +701,8 @@ def elimₛ' : (σ : Subₛ Ωₛ Γₛ) -> ConₛS Γₛ (SubₛA σ constrₛ)
 
 
 namespace Example
-  def Vec (A : Type) : Nat -> Type 1                                     := constrTmₛ' (Ω := V A) (.var .vz)
-  def Vec.nil (A : Type) : Vec A 0                                       := constrTmₚ' (Ω := V A) (.var .vz)
-  def Vec.cons (A : Type) : (n : Nat) -> (x:A) -> Vec A n -> Vec A (n+1) := constrTmₚ' (Ω := V A) (.var (.vs .vz))
-  -- def Vec.rec := elimₛ
-  -- theorem Vec.rec.nil := elimₚ
-  -- theorem Vec.rec.cons := elimₚ
+  def List (A : Type) : Type 1                         := constrTmₛ' (Ω := V A) (.var .vz)
+  def List.nil (A : Type) : List A                     := constrTmₚ' (Ω := V A) (.var .vz)
+  def List.cons (A : Type) : (x:A) -> List A -> List A := constrTmₚ' (Ω := V A) (.var (.vs .vz))
+
 end Example
